

## APPENDIX A

### SOLUTION TO PROBLEM 21

By introducing an auxiliary variable  $\nu$ , Problem 21 can be further rewritten as follows.

$$\begin{aligned} \min_{\mu, \nu} \quad & \mu^T \mathbf{M} \nu + 2\mu^T \mathbf{y} \\ \text{s.t.} \quad & \mu^T \mathbf{1} = 1, \mu \geq \mathbf{0}, \mu = \nu \end{aligned} \quad (1)$$

So, we have the following augmented Lagrangian function.

$$\begin{aligned} \min_{\mu, \nu} \quad & \mu^T \mathbf{M} \nu + 2\mu^T \mathbf{y} + \frac{\rho}{2} \left\| \mu - \nu + \frac{\eta}{\rho} \right\|_2^2 \\ \text{s.t.} \quad & \mu^T \mathbf{1} = 1, \mu \geq \mathbf{0} \end{aligned} \quad (2)$$

where  $\rho$  is the penalty parameter and  $\eta$  is the Lagrangian multiplier. Next alternate optimization will be performed.

**Step 1:** Fixing  $\mu$ , we have

$$\min_{\nu} \mu^T \mathbf{M} \nu + \frac{\rho}{2} \left\| \mu - \nu + \frac{\eta}{\rho} \right\|_2^2 \quad (3)$$

Taking derivative and setting it to zero, we know

$$\mathbf{M}^T \mu - \rho(\mu - \nu + \eta/\rho) = 0 \quad (4)$$

The solution is derived as follows.

$$\nu = \mu + (\eta - \mathbf{M}^T \mu)/\rho \quad (5)$$

**Step 2:** Fixing  $\nu$ , we have

$$\begin{aligned} \min_{\mu} \quad & \mu^T \mathbf{M} \nu + 2\mu^T \mathbf{y} + \frac{\rho}{2} \left\| \mu - \nu + \frac{\eta}{\rho} \right\|_2^2 \\ \text{s.t.} \quad & \mu^T \mathbf{1} = 1, \mu \geq \mathbf{0} \end{aligned} \quad (6)$$

Eq. (6) is equivalent to the following problem.

$$\begin{aligned} \min_{\mu} \quad & \mu^T \mu - 2\mu^T (\rho \nu - \eta - \mathbf{M} \nu - 2\mathbf{y})/\rho \\ \text{s.t.} \quad & \mu^T \mathbf{1} = 1, \mu \geq \mathbf{0} \end{aligned} \quad (7)$$

Let  $\mathbf{e} = (\rho \nu - \eta - \mathbf{M} \nu - 2\mathbf{y})/\rho$ , Eq. (7) can be further rewritten as follows.

$$\begin{aligned} \min_{\mu} \quad & \left\| \mu - \mathbf{e} \right\|_2^2 \\ \text{s.t.} \quad & \mu^T \mathbf{1} = 1, \mu \geq \mathbf{0} \end{aligned} \quad (8)$$

The Lagrangian function of Eq. (8) is

$$\mathcal{L}(\mu, \zeta, \xi) = \frac{1}{2} \left\| \mu - \mathbf{e} \right\|_2^2 - \zeta(\mu^T \mathbf{1} - 1) - \xi^T \mu \quad (9)$$

According to the KKT conditions, we have

$$\mu_i^* = (z_i - \bar{\xi}^*)_+ \quad (10)$$

$$\xi_i^* = (\bar{\xi}^* - z_i)_+ \quad (11)$$

where  $\mathbf{z} = \mathbf{e} - \frac{11^T}{n_v} \mathbf{e} + \frac{1}{n_v}$  and  $\bar{\xi}^* = \frac{1^T \xi^*}{n_v}$ . Obviously,  $\mu$  can be determined by Eq. (10) if we know  $\xi^*$ . From Eq. (11), we further know the following relationship.

$$\bar{\xi}^* = \frac{1}{n_v} \sum_{i=1}^{n_v} (\bar{\xi}^* - z_i)_+ \quad (12)$$

Defining a function as

$$f(\bar{\xi}) = \frac{1}{n_v} \sum_{i=1}^{n_v} (\bar{\xi} - z_i)_+ - \bar{\xi} \quad (13)$$

we can obtain  $\bar{\xi}^*$  by the root-finding problem  $f(\bar{\xi}^*) = 0$ . This problem can be solved efficiently by Newton method (14), requiring only 2-4 iterations.

$$\bar{\xi}_{t+1} = \bar{\xi}_t - \frac{f(\bar{\xi}_t)}{f'(\bar{\xi}_t)} \quad (14)$$

**Step 3:** Get a more accurate multiplier by  $\eta = \eta + \rho(\mu - \nu)$ .

**Step 4:** Increase the penalty parameter by  $\rho = \tau \rho$ .

In a nutshell, Problem 21 can be solved through the above four steps.

## APPENDIX B

### DERIVATION OF EQUATIONS 10 AND 11

For any  $i$ , Eq. (9) has the following KKT conditions:

$$\mu_i^* - e_i - \zeta^* - \xi_i^* = 0 \quad (15)$$

$$\xi_i^* \mu_i^* = 0 \quad (16)$$

$$\mu_i^* \geq 0 \quad (17)$$

$$\xi_i^* \geq 0 \quad (18)$$

According to  $\mathbf{1}^T \mu^* = 1$  and Eq. (15), we know

$$\zeta^* = (1 - \mathbf{1}^T \mathbf{e} - \mathbf{1}^T \xi^*)/n_v \quad (19)$$

Combining Eq. (15) and Eq. (19), we have

$$\mu_i^* = z_i - \bar{\xi}^* + \xi_i^* \quad (20)$$

where  $\mathbf{z} = \mathbf{e} - \frac{11^T}{n_v} \mathbf{e} + \frac{1}{n_v}$  and  $\bar{\xi}^* = \frac{1^T \xi^*}{n_v}$ . Following Eqs. (16)-(18) and (20), Eqs. (10) and (11) hold.